ulib/experimental/Steel.ST.HigherArray.fsti
@@ -43,6 +43,10 @@ val base_len (#elt: Type) (b: base_t elt) : GTot nat
 val ptr ([@@@strictly_positive] elt: Type u#a) : Type0
 [@@noextract_to "krml"]
 val null_ptr (elt: Type u#a) : ptr elt
+// TODO: turn into a stateful operation to avoid comparing dangling pointers
+val is_null_ptr (#elt: Type u#a) (p: ptr elt) : Pure bool
+  (requires True)
+  (ensures (fun res -> res == true <==> p == null_ptr elt))
 val base (#elt: Type) (p: ptr elt) : Tot (base_t elt)
 val offset (#elt: Type) (p: ptr elt) : Ghost nat (requires True) (ensures (fun offset -> offset <= base_len (base p)))
 val ptr_base_offset_inj (#elt: Type) (p1 p2: ptr elt) : Lemma
